test: PCF with references — clean file with 5 Admitted to prove

mcp-coq-lsp/test_issues.v
@@ -1,37 +1,46 @@
 Require Import Arith List Compare_dec.
 Import ListNotations.
 
+(** * PCF with References *)
+
 Inductive ty : Type :=
-  | TyNat : ty | TyBool : ty | TyArrow : ty -> ty -> ty.
+  | TyNat | TyBool | TyArrow : ty -> ty -> ty | TyRef : ty -> ty.
 
 Inductive tm : Type :=
   | Var : nat -> tm | Num : nat -> tm | BOOL : bool -> tm
   | Succ : tm -> tm | Pred : tm -> tm | IsZero : tm -> tm
   | If : tm -> tm -> tm -> tm
-  | Lam : ty -> tm -> tm | App : tm -> tm -> tm | Fix : tm -> tm.
+  | Lam : ty -> tm -> tm | App : tm -> tm -> tm | Fix : tm -> tm
+  | Ref : tm -> tm | Deref : tm -> tm | Assign : tm -> tm -> tm
+  | Loc : nat -> tm.
 
 Definition ctx := list ty.
+Definition store_ty := list ty.
 
-Inductive has_type : ctx -> tm -> ty -> Prop :=
-  | T_Var : forall G x T, nth_error G x = Some T -> has_type G (Var x) T
-  | T_Num : forall G n, has_type G (Num n) TyNat
-  | T_Bool : forall G b, has_type G (BOOL b) TyBool
-  | T_Succ : forall G t, has_type G t TyNat -> has_type G (Succ t) TyNat
-  | T_Pred : forall G t, has_type G t TyNat -> has_type G (Pred t) TyNat
-  | T_IsZero : forall G t, has_type G t TyNat -> has_type G (IsZero t) TyBool
-  | T_If : forall G t1 t2 t3 T,
-      has_type G t1 TyBool -> has_type G t2 T -> has_type G t3 T -> has_type G (If t1 t2 t3) T
-  | T_Lam : forall G T1 T2 t,
-      has_type (T1 :: G) t T2 -> has_type G (Lam T1 t) (TyArrow T1 T2)
-  | T_App : forall G t1 t2 T1 T2,
-      has_type G t1 (TyArrow T1 T2) -> has_type G t2 T1 -> has_type G (App t1 t2) T2
-  | T_Fix : forall G t T,
-      has_type (T :: G) t T -> has_type G (Fix t) T.
+Inductive has_type : ctx -> store_ty -> tm -> ty -> Prop :=
+  | T_Var : forall G S x T, nth_error G x = Some T -> has_type G S (Var x) T
+  | T_Num : forall G S n, has_type G S (Num n) TyNat
+  | T_Bool : forall G S b, has_type G S (BOOL b) TyBool
+  | T_Succ : forall G S t, has_type G S t TyNat -> has_type G S (Succ t) TyNat
+  | T_Pred : forall G S t, has_type G S t TyNat -> has_type G S (Pred t) TyNat
+  | T_IsZero : forall G S t, has_type G S t TyNat -> has_type G S (IsZero t) TyBool
+  | T_If : forall G S t1 t2 t3 T,
+      has_type G S t1 TyBool -> has_type G S t2 T -> has_type G S t3 T -> has_type G S (If t1 t2 t3) T
+  | T_Lam : forall G S T1 T2 t,
+      has_type (T1 :: G) S t T2 -> has_type G S (Lam T1 t) (TyArrow T1 T2)
+  | T_App : forall G S t1 t2 T1 T2,
+      has_type G S t1 (TyArrow T1 T2) -> has_type G S t2 T1 -> has_type G S (App t1 t2) T2
+  | T_Fix : forall G S t T,
+      has_type (T :: G) S t T -> has_type G S (Fix t) T
+  | T_Ref : forall G S t T, has_type G S t T -> has_type G S (Ref t) (TyRef T)
+  | T_Deref : forall G S t T, has_type G S t (TyRef T) -> has_type G S (Deref t) T
+  | T_Assign : forall G S t1 t2 T,
+      has_type G S t1 (TyRef T) -> has_type G S t2 T -> has_type G S (Assign t1 t2) TyNat
+  | T_Loc : forall G S l T, nth_error S l = Some T -> has_type G S (Loc l) (TyRef T).
 
 Inductive value : tm -> Prop :=
-  | V_Num : forall n, value (Num n)
-  | V_Bool : forall b, value (BOOL b)
-  | V_Lam : forall T t, value (Lam T t).
+  | V_Num : forall n, value (Num n) | V_Bool : forall b, value (BOOL b)
+  | V_Lam : forall T t, value (Lam T t) | V_Loc : forall l, value (Loc l).
 
 Fixpoint subst (j : nat) (s : tm) (t : tm) : tm :=
   match t with
@@ -43,51 +52,96 @@ Fixpoint subst (j : nat) (s : tm) (t : tm) : tm :=
   | Lam T t1 => Lam T (subst (S j) s t1)
   | App t1 t2 => App (subst j s t1) (subst j s t2)
   | Fix t1 => Fix (subst (S j) s t1)
+  | Ref t1 => Ref (subst j s t1) | Deref t1 => Deref (subst j s t1)
+  | Assign t1 t2 => Assign (subst j s t1) (subst j s t2)
+  | Loc l => Loc l
   end.
 
-Inductive step : tm -> tm -> Prop :=
-  | S_Succ : forall t t', step t t' -> step (Succ t) (Succ t')
-  | S_PredZero : step (Pred (Num 0)) (Num 0)
-  | S_PredSucc : forall n, step (Pred (Num (S n))) (Num n)
-  | S_Pred : forall t t', step t t' -> step (Pred t) (Pred t')
-  | S_IsZeroZero : step (IsZero (Num 0)) (BOOL true)
-  | S_IsZeroSucc : forall n, step (IsZero (Num (S n))) (BOOL false)
-  | S_IsZero : forall t t', step t t' -> step (IsZero t) (IsZero t')
-  | S_IfTrue : forall t1 t2, step (If (BOOL true) t1 t2) t1
-  | S_IfFalse : forall t1 t2, step (If (BOOL false) t1 t2) t2
-  | S_If : forall t1 t1' t2 t3, step t1 t1' -> step (If t1 t2 t3) (If t1' t2 t3)
-  | S_App1 : forall t1 t1' t2, step t1 t1' -> step (App t1 t2) (App t1' t2)
-  | S_App2 : forall v1 t2 t2', value v1 -> step t2 t2' -> step (App v1 t2) (App v1 t2')
-  | S_AppAbs : forall T t1 v2, value v2 -> step (App (Lam T t1) v2) (subst 0 v2 t1)
-  | S_Fix : forall t, step (Fix t) (subst 0 (Fix t) t).
+Definition heap := list (nat * tm).
+
+Fixpoint heap_lookup (l : nat) (mu : heap) : option tm :=
+  match mu with | [] => None | (l',v)::mu' => if Nat.eqb l l' then Some v else heap_lookup l mu' end.
+
+Fixpoint heap_update (l : nat) (v : tm) (mu : heap) : heap :=
+  match mu with | [] => [] | (l',v')::mu' => if Nat.eqb l l' then (l,v)::mu' else (l',v') :: heap_update l v mu' end.
+
+Inductive heap_ok : heap -> store_ty -> Prop :=
+  | heap_empty : forall S, heap_ok [] S
+  | heap_cons : forall l v mu S T,
+      heap_ok mu S -> has_type [] S v T -> nth_error S l = Some T ->
+      heap_ok ((l, v) :: mu) S.
+
+Inductive step : tm -> heap -> tm -> heap -> Prop :=
+  | S_Succ : forall t mu t' mu', step t mu t' mu' -> step (Succ t) mu (Succ t') mu'
+  | S_PredZero : forall mu, step (Pred (Num 0)) mu (Num 0) mu
+  | S_PredSucc : forall n mu, step (Pred (Num (S n))) mu (Num n) mu
+  | S_Pred : forall t mu t' mu', step t mu t' mu' -> step (Pred t) mu (Pred t') mu'
+  | S_IsZeroZero : forall mu, step (IsZero (Num 0)) mu (BOOL true) mu
+  | S_IsZeroSucc : forall n mu, step (IsZero (Num (S n))) mu (BOOL false) mu
+  | S_IsZero : forall t mu t' mu', step t mu t' mu' -> step (IsZero t) mu (IsZero t') mu'
+  | S_IfTrue : forall t1 t2 mu, step (If (BOOL true) t1 t2) mu t1 mu
+  | S_IfFalse : forall t1 t2 mu, step (If (BOOL false) t1 t2) mu t2 mu
+  | S_If : forall t1 mu t1' mu' t2 t3, step t1 mu t1' mu' -> step (If t1 t2 t3) mu (If t1' t2 t3) mu'
+  | S_App1 : forall t1 mu t1' mu' t2, step t1 mu t1' mu' -> step (App t1 t2) mu (App t1' t2) mu'
+  | S_App2 : forall v1 t2 mu t2' mu', value v1 -> step t2 mu t2' mu' -> step (App v1 t2) mu (App v1 t2') mu'
+  | S_AppAbs : forall T t1 v2 mu, value v2 -> step (App (Lam T t1) v2) mu (subst 0 v2 t1) mu
+  | S_Fix : forall t mu, step (Fix t) mu (subst 0 (Fix t) t) mu
+  | S_Ref : forall t mu t' mu', step t mu t' mu' -> step (Ref t) mu (Ref t') mu'
+  | S_RefV : forall v mu, value v -> step (Ref v) mu (Loc (length mu)) ((length mu, v) :: mu)
+  | S_Deref : forall t mu t' mu', step t mu t' mu' -> step (Deref t) mu (Deref t') mu'
+  | S_DerefLoc : forall l mu v, heap_lookup l mu = Some v -> step (Deref (Loc l)) mu v mu
+  | S_Assign1 : forall t1 mu t1' mu' t2, step t1 mu t1' mu' -> step (Assign t1 t2) mu (Assign t1' t2) mu'
+  | S_Assign2 : forall l t2 mu t2' mu', step t2 mu t2' mu' -> step (Assign (Loc l) t2) mu (Assign (Loc l) t2') mu'
+  | S_AssignV : forall l v mu, value v -> step (Assign (Loc l) v) mu (Num 0) (heap_update l v mu).
 
 Lemma ctx_lookup_app : forall G1 G2 x T,
-  nth_error (G1 ++ G2) (length G1 + x) = Some T ->
-  nth_error G2 x = Some T.
-Proof.
-  induction G1; simpl; intros H; [exact H | apply IHG1; exact H].
-Qed.
+  nth_error (G1 ++ G2) (length G1 + x) = Some T -> nth_error G2 x = Some T.
+Proof. induction G1; simpl; intros H; [exact H | apply IHG1; exact H]. Qed.
 
 Lemma ctx_lookup_skip : forall G1 G2 x T,
-  nth_error (G1 ++ (T :: G2)) x = Some T ->
-  x < length G1 ->
-  nth_error G1 x = Some T.
+  nth_error (G1 ++ (T :: G2)) x = Some T -> x < length G1 -> nth_error G1 x = Some T.
 Proof.
-induction G1 as [| T1 G1' IH]; simpl; intros x T2 H Hlen; [exfalso; exact (Lt.lt_n_O _ Hlen) | ].
+  induction G1 as [| T1 G1' IH]; simpl; intros x T2 H Hlen;
+    [exfalso; exact (Lt.lt_n_O _ Hlen) | ].
 Qed.
 
-
-Lemma substitution_preserves_typing : forall G1 G2 x s t T,
-    has_type (G1 ++ (T :: G2)) t T ->
-  has_type (G1 ++ G2) (subst (length G1) s t) T.
+Lemma substitution_preserves_typing : forall G1 G2 S x s t T,
+  has_type (G1 ++ G2) S s T ->
+  has_type (G1 ++ (T :: G2)) S t T ->
+  has_type (G1 ++ G2) S (subst (length G1) s t) T.
 Proof.
-intros G1 G2 x s t T Hs Ht. revert G1 G2 x s Hs. induction Ht; simpl; intros G1 G2 x s Hs.
+  intros G1 G2 S x s t T Hs Ht. revert G1 G2 x s Hs.
+  induction Ht; simpl; intros G1 G2 x s Hs.
 Qed.
 
+Definition extends (S' S : store_ty) : Prop := exists S2, S' = S ++ S2.
+Lemma extends_refl : forall S, extends S S.
+Proof. exists []; rewrite app_nil_r; reflexivity. Qed.
 
-Theorem preservation : forall t t' T,
-  has_type [] t T -> step t t' -> has_type [] t' T.
+Lemma nth_error_app_l : forall A (l1 l2 : list A) n x,
+  nth_error l1 n = Some x -> nth_error (l1 ++ l2) n = Some x.
 Proof.
-intros t t' T Ht Hstep. revert T Ht. induction Hstep; intros T Ht; inversion Ht; subst; eauto; try (constructor; eauto).
-Qed.
+Admitted.
 
+Lemma has_type_weaken : forall G S1 S2 t T,
+  has_type G S1 t T -> extends S2 S1 -> has_type G S2 t T.
+Proof.
+Admitted.
+
+Lemma extends_heap_ok : forall mu S S',
+  heap_ok mu S -> extends S' S -> heap_ok mu S'.
+Proof.
+Admitted.
+
+Lemma heap_ok_lookup : forall mu S l v,
+  heap_ok mu S -> heap_lookup l mu = Some v ->
+  exists T, nth_error S l = Some T /\ has_type [] S v T.
+Proof.
+Admitted.
+
+Theorem preservation : forall t mu t' mu' T S,
+  has_type [] S t T -> step t mu t' mu' ->
+  heap_ok mu S ->
+  exists S', extends S' S /\ heap_ok mu' S' /\ has_type [] S' t' T.
+Proof.
+Admitted.
